fix client03 thread1 proof

src/example/Client03.v
@@ -41,7 +41,6 @@ Module Client03.
       fun _ =>
         _ <- trigger Yield;;
         let a := (0 : nat) in
-        (* a <- Ret (0 : nat);; *)
         _ <- (ITree.iter (fun (i : nat) =>
                            r <- (if (Nat.eq_dec i 100)
                                 then Ret (inr tt)
@@ -63,7 +62,6 @@ Module Client03.
       fun _ =>
         _ <- trigger Yield;;
         let a := (0 : nat) in
-        (* a <- Ret (0 : nat);; *)
         _ <- (ITree.iter (fun (i : nat) =>
                            r <- (if (Nat.eq_dec i 10)
                                 then Ret (inr tt)
@@ -141,14 +139,11 @@ Section SPEC.
 
   (* Namespace for Client03 invariants. *)
   Definition N_Client03 : namespace := (nroot .@ "Client03").
-  Definition N_counter_inv : namespace := (N_Client03 .@ "counter").
   Definition N_t2_write_inv : namespace := (N_Client03 .@ "t2_write").
+  Definition N_t2_promise_inv : namespace := (N_Client03 .@ "t2_promise").
 
   Definition counter n c1 c2 r1 r2 : Formula n :=
     (∃ (x y : τ{nat}), (C ↦ ((c1 * x) + (c2 * y))) ∗ ➢(auexa_b r1 (x : nat)) ∗ ➢(auexa_b r2 (y : nat)))%F.
-
-  (* Definition counter_inv n r1 r2 : Formula n := *)
-  (*   (syn_inv n N_counter_inv (counter n r1 r2)). *)
 
   Definition t2_write n r : Formula n :=
     (➢(auexa_w r (10 : nat)) ∗ (D ↦ 1))%F.
@@ -156,27 +151,36 @@ Section SPEC.
   Definition t2_write_inv n r : Formula n :=
     (syn_inv n N_t2_write_inv (t2_write n r))%F.
 
+  Definition t2_promise n w r : Formula n :=
+    ((D ↦ 0) -U-[w](0)-◇ (t2_write_inv n r))%F.
+
+  Definition t2_promise_inv n w r : Formula n :=
+    (syn_inv n N_t2_promise_inv (t2_promise n w r))%F.
+
   (** Simulation proof. *)
 
   Lemma Client03_incr_spec
-        tid N Es c1 c2
+        tid N Es
         (TOP : OwnEs_top Es)
     :
-    ⊢ ∀ (r k lft l r1 r2 a : τ{nat, 1+N}) (ds : list (nat * nat * Formula N)),
+    ⊢ ∀ (r k lft l r1 r2 a c1 c2 c0 r0 : τ{nat, 1+N}) (ds : list (nat * nat * Formula N))
+      ,
         [@ tid, N, Es @]
           ⧼⟦((syn_tgt_interp_as N sndl (λ m : SCMem.t, ➢(scm_memory_black m)))
-               ∗ (⤉ Duty(tid) ds) ∗ ◇{List.map fst ds}(lft, 1) ∗ ◇{List.map fst ds}(0, 1)
-               ∗ ◇{List.map fst ds}(0, 5)
+               ∗ (⤉ Duty(tid) ds) ∗ ◇{List.map fst ds}(lft, 1) ∗ ◇{List.map fst ds}(0, 6)
                ∗ (⤉ isSpinlock N r L (counter N c1 c2 r1 r2) k lft l)
                ∗ (⌜2 <= l⌝) ∗ live[k] (1/2) ∗ ◇[k](1+l, 1)
-               ∗ ➢(auexa_w r1 (a : nat)))%F , 1+N⟧⧽
-            (OMod.close_itree omod (SCMem.mod gvs) (incr c1))
-            ⧼rv, ⟦((⤉ Duty(tid) ds) ∗ live[k] (1/2) ∗  ➢(auexa_w r1 (a + 1)))%F, 1+N⟧⧽
+               ∗ ➢(auexa_w r0 (a : nat))
+               ∗ ⌜(r0 = r1 /\ c0 = c1) \/ (r0 = r2 /\ c0 = c2)⌝
+            )%F, 1+N⟧⧽
+            (OMod.close_itree omod (SCMem.mod gvs) (incr c0))
+            ⧼rv, ⟦((⤉ Duty(tid) ds) ∗ live[k] (1/2) ∗  ➢(auexa_w r0 (a + 1)))%F, 1+N⟧⧽
   .
   Proof.
     iIntros. simpl. iStartTriple.
     red_tl. simpl. rewrite red_syn_tgt_interp_as.
-    iIntros "(#MEM & DUTY & PCS_SPIN1 & PCS_SPIN2 & PCS & #ISL & %LE & LIVE_k & PC_k & CNTW_r1)".
+    iIntros "(#MEM & DUTY & PCS_SPIN1 & PCS & #ISL & %LE & LIVE_k & PC_k & CNTW_r0 & %CASES)".
+    iMod (pcs_decr _ _ 5 1 with "PCS") as "[PCS PCS_SPIN2]". lia.
     iIntros "POST".
     unfold incr. rred.
     iMod (pcs_decr _ _ 4 1 with "PCS") as "[PCS PCS1]". auto.
@@ -184,7 +188,7 @@ Section SPEC.
     2:{ iFrame. }
     auto.
     iIntros "DUTY _". iModIntro. rred2r. iApply wpsim_tauR. rred2r.
-    iApply (Spinlock_lock_spec with "[LIVE_k DUTY PCS_SPIN1 PCS_SPIN2] [PCS PC_k CNTW_r1 POST]").
+    iApply (Spinlock_lock_spec with "[LIVE_k DUTY PCS_SPIN1 PCS_SPIN2] [PCS PC_k CNTW_r0 POST]").
     1,2: ss.
     { red_tl. simpl. rewrite red_syn_tgt_interp_as. iSplit. eauto. iSplitR. eauto. iFrame. }
     iEval (red_tl). iIntros (_) "[%u A]". iEval (unfold counter; red_tl) in "A".
@@ -221,25 +225,45 @@ Section SPEC.
     2:{ iSplitL "DUTY". iFrame. simpl. iApply pcs_cons_fold. iFrame. }
     auto.
     iIntros "DUTY _". iModIntro. rred2r. iApply wpsim_tauR. rred2r.
-    replace (SCMem.val_add rv c1) with ((c1 * (1 + x) + c2 * y) : SCMem.val).
-    2:{ subst rv. ss. f_equal. lia. }
-    iPoseProof (auexa_b_w_eq with "CNTB_r1 CNTW_r1") as "%EQ". subst a.
-    iMod (auexa_b_w_update _ _ _ _ nat (1 + x) with "CNTB_r1 CNTW_r1") as "[CNTB_r1 CNTW_r1]".
-    iApply (Spinlock_unlock_spec with "[CNTB_r1 CNTB_r2 PT LOCKED LIVE_k DUTY PCS LIVE_u PC_u PC_k]").
-    3:{ repeat (try rewrite @red_tl_sepconj). simpl.
-        iSplitR. rewrite red_syn_tgt_interp_as. eauto. iSplitR. eauto.
-        unfold counter. red_tl. iSplitL "PT CNTB_r1 CNTB_r2".
-        { iExists (1+x). red_tl. iExists y. red_tl. iFrame. }
-        Local Opaque progress_credits.
-        simpl. iEval (replace (l+1) with (S l) by lia). iFrame.
-        iApply pcs_cons_fold.
-        iPoseProof (pc_split with "[PC_u]") as "[PC1 PC2]". 2: iFrame.
-        simpl. replace 97 with (96 + 1) by ss. iFrame.
-        Local Transparent progress_credits.
-    }
-    ss. ss.
-    iEval red_tl. iIntros (_) "[DUTY LIVE_k]". rred2r.
-    iApply "POST". replace (1+x) with (x+1). iFrame. lia.
+    destruct CASES as [CASE | CASE]; des; subst r0; subst c0.
+    - replace (SCMem.val_add rv c1) with ((c1 * (1 + x) + c2 * y) : SCMem.val).
+      2:{ subst rv. ss. f_equal. lia. }
+      iPoseProof (auexa_b_w_eq with "CNTB_r1 CNTW_r0") as "%EQ". subst a.
+      iMod (auexa_b_w_update _ _ _ _ nat (1 + x) with "CNTB_r1 CNTW_r0") as "[CNTB_r1 CNTW_r0]".
+      iApply (Spinlock_unlock_spec with "[CNTB_r1 CNTB_r2 PT LOCKED LIVE_k DUTY PCS LIVE_u PC_u PC_k]").
+      3:{ repeat (try rewrite @red_tl_sepconj). simpl.
+          iSplitR. rewrite red_syn_tgt_interp_as. eauto. iSplitR. eauto.
+          unfold counter. red_tl. iSplitL "PT CNTB_r1 CNTB_r2".
+          { iExists (1+x). red_tl. iExists y. red_tl. iFrame. }
+          Local Opaque progress_credits.
+          simpl. iEval (replace (l+1) with (S l) by lia). iFrame.
+          iApply pcs_cons_fold.
+          iPoseProof (pc_split with "[PC_u]") as "[PC1 PC2]". 2: iFrame.
+          simpl. replace 97 with (96 + 1) by ss. iFrame.
+          Local Transparent progress_credits.
+      }
+      ss. ss.
+      iEval red_tl. iIntros (_) "[DUTY LIVE_k]". rred2r.
+      iApply "POST". replace (1+x) with (x+1). iFrame. lia.
+    - replace (SCMem.val_add rv c2) with ((c1 * x + c2 * (1 + y)) : SCMem.val).
+      2:{ subst rv. ss. f_equal. lia. }
+      iPoseProof (auexa_b_w_eq with "CNTB_r2 CNTW_r0") as "%EQ". subst a.
+      iMod (auexa_b_w_update _ _ _ _ nat (1 + y) with "CNTB_r2 CNTW_r0") as "[CNTB_r2 CNTW_r0]".
+      iApply (Spinlock_unlock_spec with "[CNTB_r1 CNTB_r2 PT LOCKED LIVE_k DUTY PCS LIVE_u PC_u PC_k]").
+      3:{ repeat (try rewrite @red_tl_sepconj). simpl.
+          iSplitR. rewrite red_syn_tgt_interp_as. eauto. iSplitR. eauto.
+          unfold counter. red_tl. iSplitL "PT CNTB_r1 CNTB_r2".
+          { iExists x. red_tl. iExists (1+y). red_tl. simpl. iFrame. }
+          Local Opaque progress_credits.
+          simpl. iEval (replace (l+1) with (S l) by lia). iFrame.
+          iApply pcs_cons_fold.
+          iPoseProof (pc_split with "[PC_u]") as "[PC1 PC2]". 2: iFrame.
+          simpl. replace 97 with (96 + 1) by ss. iFrame.
+          Local Transparent progress_credits.
+      }
+      ss. ss.
+      iEval red_tl. iIntros (_) "[DUTY LIVE_k]". rred2r.
+      iApply "POST". replace (1+y) with (y+1). iFrame. lia.
   Qed.
 
   Local Opaque incr.
@@ -256,7 +280,7 @@ Section SPEC.
                ∗ ◇[k](3, 101)
                ∗ ➢(auexa_w r1 0)
                ∗ ◆[w, wl]
-               ∗ (⤉ ((D ↦ 0) -U-[w](0)-◇ (t2_write_inv N r2)))
+               ∗ (⤉ t2_promise_inv N w r2)
             )
               -∗
               syn_wpsim (1+N) tid ∅
@@ -265,10 +289,11 @@ Section SPEC.
               (fn2th Client03Spec.module "thread1" (tt ↑))
               (fn2th Client03.module "thread1" (tt ↑)))%F, 1+N⟧.
   Proof.
-    iIntros. simpl. red_tl; iIntros (r). red_tl. iIntros (k). red_tl. iIntros (w). red_tl. iIntros (wl). red_tl. iIntros (r1). red_tl. iIntros (r2).
+    iIntros. simpl.
+    red_tl; iIntros (r). red_tl. iIntros (k). red_tl. iIntros (w). red_tl. iIntros (wl). red_tl. iIntros (r1). red_tl. iIntros (r2).
     red_tl. simpl.
-    rewrite red_syn_tgt_interp_as. rewrite red_syn_until_tpromise. rewrite red_syn_wpsim.
-    iIntros "(#MEM & TID & DUTY & #ISL & LIVE_k & PC_k & CNTW_r1 & #LO_w & UNTIL)".
+    rewrite red_syn_tgt_interp_as. unfold t2_promise_inv. rewrite red_syn_inv. rewrite red_syn_wpsim.
+    iIntros "(#MEM & TID & DUTY & #ISL & LIVE_k & PC_k & CNTW_r1 & #LO_w & #UNTILI)".
     unfold fn2th. simpl. lred2r. rred2r.
     iApply (wpsim_yieldR with "[DUTY]").
     2:{ iSplitL "DUTY". iApply "DUTY". simpl. ss. }
@@ -293,18 +318,17 @@ Section SPEC.
     assert (LT : j <= 100). subst. lia.
     clear H0 H.
     iStopProof.
-    (* iRevert "MEM ISL TID LIVE_k PC_k CNTW_r1 UNTIL DUTY". iStopProof. *)
     revert j HeqJ LT. induction J; cycle 1.
-    { i. iIntros "((#MEM & #ISL & #LO_w) & TID & LIVE_k & PC_k & CNTW_r1 & UNTIL & DUTY)".
+    { i. iIntros "((#MEM & #ISL & #LO_w & #UNTILI) & TID & LIVE_k & PC_k & CNTW_r1 & DUTY)".
       iEval (rewrite unfold_iter_eq). rred2r.
       destruct (Nat.eq_dec j 100).
       { exfalso. lia. }
       rred2.
       iPoseProof (pc_split _ _ 1 (S J) with "PC_k") as "[PC_k1 PC_k]".
-      iApply (Client03_incr_spec with "[DUTY LIVE_k PC_k1 CNTW_r1] [TID UNTIL PC_k]").
+      iApply (Client03_incr_spec with "[DUTY LIVE_k PC_k1 CNTW_r1] [TID PC_k]").
       ss.
       { red_tl. simpl. iSplitR. rewrite red_syn_tgt_interp_as. eauto. iFrame.
-        simpl. do 3 (iSplitR; [iApply pcs_nil |]). iSplit. eauto. auto.
+        simpl. do 2 (iSplitR; [iApply pcs_nil |]). iSplit. eauto. iSplit; eauto.
       }
       iEval red_tl. iIntros (_) "(DUTY & LIVE_k & CNTW_r1)". rred2r.
       iApply (wpsim_yieldR with "[DUTY]").
@@ -313,54 +337,68 @@ Section SPEC.
       iIntros "DUTY _". iModIntro. rred2r. iApply wpsim_tauR. rred2r.
       iApply wpsim_tauR.
       specialize (IHJ (j+1)).
-      iPoseProof (IHJ with "[TID LIVE_k PC_k CNTW_r1 UNTIL DUTY]") as "IH".
-      (* iPoseProof (IHJ with "[] MEM ISL TID LIVE_k PC_k CNTW_r1 UNTIL DUTY") as "IH". *)
+      iPoseProof (IHJ with "[TID LIVE_k PC_k CNTW_r1 DUTY]") as "IH".
       { lia. }
       { lia. }
       { iSplit. iModIntro. eauto. iFrame. }
       iApply "IH".
     }
-    i. iIntros "((#MEM & #ISL & #LO_w) & TID & LIVE_k & PC_k & CNTW_r1 & UNTIL & DUTY)".
+    i. iIntros "((#MEM & #ISL & #LO_w & #UNTILI) & TID & LIVE_k & PC_k & CNTW_r1 & DUTY)".
     iEval (rewrite unfold_iter_eq). rred2r.
     destruct (Nat.eq_dec j 100).
     2:{ exfalso. lia. }
-    rred2r. iPoseProof (until_tpromise_get_tpromise with "UNTIL") as "#TPROM".
-    iRevert "TID LIVE_k PC_k CNTW_r1 DUTY".
-    iMod (until_tpromise_ind _ with "[UNTIL] []") as "IH".
+    rred2r.
+    (* Set-up for induction. *)
+    iEval (rewrite unfold_iter_eq). rred2r.
+    iApply (wpsim_yieldR with "[DUTY]").
+    2:{ iFrame. }
+    auto.
+    iIntros "DUTY _". iModIntro. rred2r.
+    iInv "UNTILI" as "UNTIL" "UNTIL_CLOSE".
+    iEval (unfold t2_promise; simpl; red_tl) in "UNTIL". iEval (rewrite red_syn_until_tpromise) in "UNTIL".
+    iPoseProof (until_tpromise_get_tpromise with "UNTIL") as "#TPROM".
+    iRevert "TID LIVE_k PC_k CNTW_r1 DUTY UNTIL_CLOSE".
+    iMod (until_tpromise_ind with "[UNTIL] []") as "IH".
     { iSplitR. eauto. iFrame. }
     2:{ iApply "IH". }
     iSplit; iModIntro.
-    { iIntros "IH". iModIntro. iIntros "CUR TID LIVE_k PC_k CNTW_r1 DUTY".
-      iEval (rewrite unfold_iter_eq). rred2r.
-      iApply (wpsim_yieldR with "[DUTY]").
-      2:{ iFrame. }
-      auto.
-      iIntros "DUTY FC". iModIntro. rred2r.
+    { iIntros "IH". iModIntro. iIntros "CUR TID LIVE_k PC_k CNTW_r1 DUTY UNTIL_CLOSE".
       iEval (simpl; red_tl; simpl) in "CUR".
       iApply (SCMem_load_fun_spec with "[CUR] [-]").
       3:{ iFrame. eauto. }
-      auto. ss.
+      auto.
+      { rewrite lookup_insert. assert (↑N_state_tgt ## (↑N_t2_promise_inv : coPset)).
+        { apply ndot_preserve_disjoint_r. apply ndot_ne_disjoint. ss. }
+        set_solver.
+      }
       iIntros (rv) "[%RVEQ PTD]". subst rv. rred2r. iApply wpsim_tauR. rred2r.
+      iMod ("UNTIL_CLOSE" with "[PTD]") as "_".
+      { unfold t2_promise. simpl. rewrite red_syn_until_tpromise. iFrame. auto. }
       iApply (wpsim_yieldR with "[DUTY]").
       2:{ iFrame. }
       auto.
-      iIntros "DUTY _". iModIntro. rred2r. iApply (SCMem_compare_fun_spec with "[] [-]").
+      iIntros "DUTY FC". iModIntro. rred2r. iApply (SCMem_compare_fun_spec with "[] [-]").
       3:{ iApply tgt_interp_as_equiv. 2: eauto. ss. iIntros. red_tl.
           ss. iSplit. iIntros "MEM"; iFrame. ss. iIntros "[MEM _]". iFrame.
       }
       auto. ss.
       iIntros (rv) "[%TRUE _]". specialize (TRUE eq_refl). subst rv. rred2r. iApply wpsim_tauR.
       rred2r. iApply wpsim_tauR.
-      iMod ("IH" with "[FC PTD]") as "IH".
-      { iFrame. auto. }
-      iApply ("IH" with "TID LIVE_k PC_k CNTW_r1 DUTY").
-    }
-    { iIntros "#PR". iIntros "TID LIVE_k PC_k CNTW_r1 DUTY".
-      iEval (unfold t2_write_inv; simpl; red_tl) in "PR". iEval (rewrite red_syn_inv) in "PR".
-      iEval (rewrite unfold_iter_eq). rred2r. iApply (wpsim_yieldR with "[DUTY]").
+      iEval (rewrite unfold_iter_eq). rred2r.
+      iApply (wpsim_yieldR with "[DUTY]").
       2:{ iFrame. }
       auto.
       iIntros "DUTY _". iModIntro. rred2r.
+      iInv "UNTILI" as "UNTIL" "UNTIL_CLOSE".
+      iEval (unfold t2_promise; simpl; red_tl) in "UNTIL". iEval (rewrite red_syn_until_tpromise) in "UNTIL".
+      iMod ("IH" with "[FC UNTIL]") as "IH".
+      { iFrame. }
+      iApply ("IH" with "TID LIVE_k PC_k CNTW_r1 DUTY UNTIL_CLOSE").
+    }
+    { iIntros "#PR". iIntros "TID LIVE_k PC_k CNTW_r1 DUTY UNTIL_CLOSE".
+      iMod ("UNTIL_CLOSE" with "[]") as "_".
+      { unfold t2_promise. simpl. rewrite red_syn_until_tpromise. iApply until_tpromise_make2. simpl. iSplit; eauto. }
+      iEval (unfold t2_write_inv; simpl; red_tl) in "PR". iEval (rewrite red_syn_inv) in "PR".
       iInv "PR" as "PRO" "PR_CLOSE". iEval (unfold t2_write; simpl; red_tl) in "PRO".
       iDestruct "PRO" as "[RES PTD]".
       iApply (SCMem_load_fun_spec with "[PTD] [-]").
@@ -444,5 +482,88 @@ Section SPEC.
       reflexivity.
     }
   Qed.
+
+  Lemma Client03_thread2_spec
+        tid N
+    :
+    ⊢ ⟦(∀ (r k w r1 r2 : τ{nat, 1+N}),
+           ((syn_tgt_interp_as N sndl (fun m => (➢ (scm_memory_black m))))
+               ∗ ○(tid)
+               ∗ (⤉ Duty(tid) [(w, 0, t2_write_inv N r2)])
+               ∗ (⤉ isSpinlock N r L (counter N 2 5 r1 r2) k 4 2)
+               ∗ live[k] (1/2)
+               ∗ ◇[k](3, 101)
+               ∗ ➢(auexa_w r2 0)
+               ∗ ◇[w](5, 1)
+               ∗ live[w] 1
+               ∗ (⤉ t2_promise_inv N w r2)
+            )
+              -∗
+              syn_wpsim (1+N) tid ∅
+              (fun rs rt => (⤉(syn_term_cond N tid _ rs rt))%F)
+              false false
+              (fn2th Client03Spec.module "thread2" (tt ↑))
+              (fn2th Client03.module "thread2" (tt ↑)))%F, 1+N⟧.
+  Proof.
+    iIntros. simpl. red_tl; iIntros (r). red_tl. iIntros (k). red_tl. iIntros (w). red_tl. iIntros (r1). red_tl. iIntros (r2).
+    red_tl. simpl.
+    rewrite red_syn_tgt_interp_as. rewrite red_syn_until_tpromise. rewrite red_syn_wpsim.
+    iIntros "(#MEM & TID & DUTY & #ISL & LIVE_k & PC_k & CNTW_r1 & #LO_w & UNTIL)".
+    unfold fn2th. simpl. lred2r. rred2r.
+    iApply (wpsim_yieldR with "[DUTY]").
+    2:{ iSplitL "DUTY". iApply "DUTY". simpl. ss. }
+    auto.
+    iIntros "DUTY _". iModIntro. rred2r. iApply wpsim_tauR. rred2r.
+    assert (exists j, 0 = j). eauto. des.
+    replace 
+      (ITree.iter
+         (λ i : nat,
+             ` r0 : nat + () <- (if Nat.eq_dec i 100 then Ret (inr ()) else incr 2;;; trigger Yield;;; Ret (inl (i + 1)));; Ret r0)
+         0)
+      with
+      (ITree.iter
+         (λ i : nat,
+             ` r0 : nat + () <- (if Nat.eq_dec i 100 then Ret (inr ()) else incr 2;;; trigger Yield;;; Ret (inl (i + 1)));; Ret r0)
+         j).
+    2:{ subst j. auto. }
+    iEval (replace 250 with ((100 * 2) + 50)).
+    remember (100 - j) as J.
+    assert (100 = J). subst. ss.
+    iEval (rewrite H0) in "PC_k". iEval (rewrite H) in "CNTW_r1".
+    assert (LT : j <= 100). subst. lia.
+    clear H0 H.
+    iStopProof.
+    (* iRevert "MEM ISL TID LIVE_k PC_k CNTW_r1 UNTIL DUTY". iStopProof. *)
+    revert j HeqJ LT. induction J; cycle 1.
+    { i. iIntros "((#MEM & #ISL & #LO_w) & TID & LIVE_k & PC_k & CNTW_r1 & UNTIL & DUTY)".
+      iEval (rewrite unfold_iter_eq). rred2r.
+      destruct (Nat.eq_dec j 100).
+      { exfalso. lia. }
+      rred2.
+      iPoseProof (pc_split _ _ 1 (S J) with "PC_k") as "[PC_k1 PC_k]".
+      iApply (Client03_incr_spec with "[DUTY LIVE_k PC_k1 CNTW_r1] [TID UNTIL PC_k]").
+      ss.
+      { red_tl. simpl. iSplitR. rewrite red_syn_tgt_interp_as. eauto. iFrame.
+        simpl. do 3 (iSplitR; [iApply pcs_nil |]). iSplit. eauto. auto.
+      }
+      iEval red_tl. iIntros (_) "(DUTY & LIVE_k & CNTW_r1)". rred2r.
+      iApply (wpsim_yieldR with "[DUTY]").
+      2:{ iSplitL "DUTY". iApply "DUTY". simpl. ss. }
+      auto.
+      iIntros "DUTY _". iModIntro. rred2r. iApply wpsim_tauR. rred2r.
+      iApply wpsim_tauR.
+      specialize (IHJ (j+1)).
+      iPoseProof (IHJ with "[TID LIVE_k PC_k CNTW_r1 UNTIL DUTY]") as "IH".
+      (* iPoseProof (IHJ with "[] MEM ISL TID LIVE_k PC_k CNTW_r1 UNTIL DUTY") as "IH". *)
+      { lia. }
+      { lia. }
+      { iSplit. iModIntro. eauto. iFrame. }
+      iApply "IH".
+    }
+    i. iIntros "((#MEM & #ISL & #LO_w) & TID & LIVE_k & PC_k & CNTW_r1 & UNTIL & DUTY)".
+    iEval (rewrite unfold_iter_eq). rred2r.
+    destruct (Nat.eq_dec j 100).
+    2:{ exfalso. lia. }
+    rred2r. iPoseProof (until_tpromise_get_tpromise with "UNTIL") as "#TPROM".
 
 End SPEC.
